Whole project compiles.  My tests show Olivier's bug (parameterized datatypes) is fixed.  Nothing new about axioms yet.

theories/L1_MalechaQuoted/program.v
@@ -55,7 +55,7 @@ Qed.
 **)
 Inductive envClass := 
 | ecTrm (_:Term)
-| ecTyp (_:itypPack)
+| ecTyp (_:nat) (_:itypPack)
 | ecAx.
 
 Lemma isAx_dec:
@@ -73,8 +73,10 @@ Proof.
   - destruct (proj1 TermTerms_dec t t0).
     + left. subst. reflexivity.
     + right. intros h. injection h. intros. contradiction.
-  - destruct (Common.RandyPrelude.list_eq_dec ityp_dec i i0).
+  - destruct (eq_nat_dec n n0), (Common.RandyPrelude.list_eq_dec ityp_dec i i0).
     + subst. left. reflexivity.
+    + right. intros h. injection h. contradiction.
+    + right. intros h. injection h. contradiction.
     + right. intros h. injection h. contradiction.
   - left. reflexivity.
 Qed.
@@ -89,7 +91,7 @@ Record Program : Type := mkPgm { main:Term; env:environ }.
 (** all items in an env are application-well-formed **)
 Inductive WFaEc: envClass -> Prop :=
 | wfaecTrm: forall t, WFapp t -> WFaEc (ecTrm t)
-| wfaecTyp: forall i, WFaEc (ecTyp i)
+| wfaecTyp: forall n i, WFaEc (ecTyp n i)
 | wfaecAx: WFaEc ecAx.
 
 Inductive WFaEnv: environ -> Prop :=
@@ -144,7 +146,7 @@ Inductive Lookup: string -> environ -> envClass -> Prop :=
 Hint Constructors Lookup.
 
 Definition LookupDfn s p t := Lookup s p (ecTrm t).
-Definition LookupTyp s p i := Lookup s p (ecTyp i).
+Definition LookupTyp s p n i := Lookup s p (ecTyp n i).
 Definition LookupAx s p := Lookup s p ecAx.
 
 Lemma Lookup_fresh_neq:
@@ -172,7 +174,7 @@ Proof.
     + left. destruct H. exists x. apply LMiss; assumption.
     + destruct e.
       * left. exists (ecTrm t). apply LHit.
-      * left. exists (ecTyp i). apply LHit. 
+      * left. exists (ecTyp n i). apply LHit. 
       * left. exists ecAx. apply LHit.
     + right. intros t h. inversion_Clear h. 
       * elim n. reflexivity.
@@ -328,7 +330,7 @@ Inductive Crct: environ -> nat -> Term -> Prop :=
 | CrctWkTrmTrm: forall n p t s nm, Crct p n t -> Crct p n s ->
            fresh nm p -> Crct ((nm,ecTrm s)::p) n t
 | CrctWkTrmTyp: forall n p t s nm, Crct p n t -> CrctTyp p n s ->
-           fresh nm p -> Crct ((nm,ecTyp s)::p) n t
+           fresh nm p -> forall m, Crct ((nm,ecTyp m s)::p) n t
 | CrctRel: forall n m p, m < n -> Crct p n prop -> Crct p n (TRel m)
 | CrctCast: forall n p t ck ty, Crct p n t -> Crct p n ty ->
                                 Crct p n (TCast t ck ty)
@@ -344,8 +346,8 @@ Inductive Crct: environ -> nat -> Term -> Prop :=
              Crct p n (TApp fn a args)
 | CrctConst: forall n p pd nm,
                Crct p n prop -> LookupDfn nm p pd -> Crct p n (TConst nm)
-| CrctConstruct: forall n p ipkgNm itypk inum cnum,
-                   Crct p n prop -> LookupTyp ipkgNm p itypk ->
+| CrctConstruct: forall n p ipkgNm npars itypk inum cnum,
+                   Crct p n prop -> LookupTyp ipkgNm p npars itypk ->
                    CrctCnstr itypk inum cnum ->
                    Crct p n (TConstruct (mkInd ipkgNm inum) cnum)
 | CrctCase: forall n p m ty mch brs,
@@ -369,7 +371,7 @@ with CrctTyp: environ -> nat -> itypPack -> Prop :=
 | CrctTypWk1: forall n p t s nm, CrctTyp p n t -> Crct p n s ->
            fresh nm p -> CrctTyp ((nm,ecTrm s)::p) n t
 | CrctTypWk2: forall n p t s nm, CrctTyp p n t -> CrctTyp p n s ->
-           fresh nm p -> CrctTyp ((nm,ecTyp s)::p) n t.
+           fresh nm p -> forall m, CrctTyp ((nm,ecTyp m s)::p) n t.
 Hint Constructors Crct Crcts CrctDs CrctTyp.
 Scheme Crct_ind' := Minimality for Crct Sort Prop
   with Crcts_ind' := Minimality for Crcts Sort Prop
@@ -458,7 +460,7 @@ Qed.
 
 Lemma CrctTypTl:
   forall pp n t, Crct pp n t ->
-             forall nm tp p, pp = ((nm,ecTyp tp)::p) -> CrctTyp p n tp.
+   forall nm npars tp p, pp = ((nm,ecTyp npars tp)::p) -> CrctTyp p n tp.
 induction 1; intros; try discriminate;
 try (solve [eapply IHCrct2; eassumption]);
 try (solve [eapply IHCrct; eassumption]).
@@ -629,27 +631,27 @@ Lemma  Crct_weaken:
 eapply CrctCrctsCrctDsTyp_ind; intros; intuition.
 - apply CrctWkTrmTrm; try assumption. eapply CrctConst; try eassumption.
 - eapply CrctConstruct; try eassumption.
-  apply H0; try assumption. apply Lookup_weaken; assumption.
+  apply H0; try assumption. apply Lookup_weaken; eassumption.
 Qed.
 
 Lemma  Crct_Typ_weaken:
   (forall p n t, Crct p n t -> 
     forall nm itp, fresh nm p -> CrctTyp p n itp ->
-                   Crct ((nm,ecTyp itp)::p) n t) /\
+                   forall npars, Crct ((nm,ecTyp npars itp)::p) n t) /\
   (forall p n ts, Crcts p n ts -> 
     forall nm itp, fresh nm p -> CrctTyp p n itp ->
-                 Crcts ((nm,ecTyp itp)::p) n ts) /\
+                 forall npars, Crcts ((nm,ecTyp npars itp)::p) n ts) /\
   (forall p n ds, CrctDs p n ds -> 
     forall nm itp, fresh nm p -> CrctTyp p n itp ->
-                   CrctDs ((nm,ecTyp itp)::p) n ds) /\
+                   forall npars, CrctDs ((nm,ecTyp npars itp)::p) n ds) /\
   (forall p n jtp, CrctTyp p n jtp -> 
     forall nm itp, fresh nm p -> CrctTyp p n itp ->
-                   CrctTyp ((nm,ecTyp itp)::p) n jtp).
+                  forall npars,  CrctTyp ((nm,ecTyp npars itp)::p) n jtp).
 Proof.
   eapply CrctCrctsCrctDsTyp_ind; intros; auto.
   - apply CrctWkTrmTyp; try assumption. eapply CrctConst; try eassumption.
   - eapply CrctConstruct; try eassumption.
-    apply H0; try assumption. apply Lookup_weaken; assumption.
+    apply H0; try assumption. apply Lookup_weaken; eassumption.
 Qed.
 
 Lemma Crct_strengthen:
@@ -772,7 +774,7 @@ Lemma Crct_invrt_Rel:
 Proof.
   induction 1; intros; try discriminate.
   - assert (j:= IHCrct1 m). intuition.
-  - assert (j:= IHCrct m). intuition.
+  - assert (j:= IHCrct m). specialize (IHCrct _ H2). intuition.
   - assert (j:= IHCrct m). injection H1. intuition.
 Qed.
 
@@ -913,16 +915,17 @@ Lemma Crct_invrt_Construct:
   forall p n construct, Crct p n construct ->
   forall ipkgNm inum cnum, construct = (TConstruct (mkInd ipkgNm inum) cnum) ->
     Crct p n prop /\
-    exists itypk, LookupTyp ipkgNm p itypk /\ CrctCnstr itypk inum cnum.
+    exists npars itypk,
+      LookupTyp ipkgNm p npars itypk /\ CrctCnstr itypk inum cnum.
 induction 1; intros; try discriminate.
 - assert (j:= IHCrct1 _ _ _ H2). intuition.
-  destruct H4 as [itypk [h1 h2]]. exists itypk. intuition.
+  destruct H4 as [npars [itypk [h1 h2]]]. exists npars, itypk. intuition.
   apply Lookup_weaken; trivial.
 - assert (j:= IHCrct _ _ _ H2). intuition.
-  destruct H4 as [itypk [h1 h2]]. exists itypk. intuition.
+  destruct H4 as [npars [itypk [h1 h2]]]. exists npars, itypk. intuition.
   apply Lookup_weaken; trivial.
 - injection H2; intros; subst. intuition.
-  exists itypk. intuition.
+  exists npars, itypk. intuition.
 Qed.
 
 Lemma Crct_App_fn_notApp:
@@ -1004,7 +1007,7 @@ Proof.
   - apply CrctInd. eapply Crct_Sort. eassumption.
   - destruct ind. edestruct (Crct_invrt_Construct H0).
     + reflexivity.
-    + destruct H3 as [x [h1 h2]]. eapply CrctConstruct; try eassumption.
+    + destruct H3 as [npars [x [h1 h2]]]. eapply CrctConstruct; try eassumption.
       * eapply Crct_Sort. eassumption.
   - destruct (Crct_invrt_Case H3 eq_refl) as [h1 [h2 h3]]. apply CrctCase.
     + apply H; trivial.
